progress on optimization example

examples/Bisimulations/optimization/optimization2.v
@@ -26,7 +26,6 @@ Open Scope string.
     TODO paragraph on linked lists and arrays
 *)
 
-
 (* First example *)
 Section ContractOptimization.
 Context { Base : ChainBase }.
@@ -71,8 +70,9 @@ Section ContractUsingArray.
     Definition result_arr := result (owners_arr * list ActionBody) error.
 
     Definition add_owner_arr (a : N) (st : owners_arr) : result_arr :=
+        if in_dec N.eq_dec a st then Err error_LINK_NOT_FOUND else
         Ok (a :: st, []).
-    
+
     Definition remove_owner_arr (a : N) (st : owners_arr) : result_arr :=
         Ok (List.remove N.eq_dec a st, []).
 
@@ -99,37 +99,110 @@ Section ContractUsingArray.
     Definition C_arr : Contract setup entrypoint owners_arr error :=
         build_contract init_arr receive_arr.
 
+    Section Aux.
+        Lemma add_owner_arr_no_acts : forall a st st' acts,
+            add_owner_arr a st = Ok (st', acts) -> acts = [].
+        Proof.
+            intros * H_add.
+            unfold add_owner_arr in H_add.
+            destruct (in_dec N.eq_dec a st) in H_add; try inversion H_add.
+            now inversion H_add.
+        Qed.
+
+        Lemma swap_owner_arr_no_acts : forall a_fst a_snd st st' acts,
+            swap_owners_arr a_fst a_snd st = Ok (st', acts) -> acts = [].
+        Proof.
+            intros * H_swap.
+            unfold swap_owners_arr in H_swap.
+            inversion H_swap as [[H_swap0 H_swap1]].
+            now subst.
+        Qed.
+
+        Lemma swap_always_succeeds : forall a_fst a_snd st,
+            exists st', swap_owners_arr a_fst a_snd st = Ok (st', []).
+        Proof.
+            intros.
+            exists (List.map (fun o => if N.eqb o a_fst then a_snd else o) st).
+            now simpl.
+        Qed.
+        
+    End Aux.
+
 End ContractUsingArray.
 
 (* the contract that uses linked lists, owners_ll *)
 Section ContractUsingLinkedList.
-    Section Aux.
-        Definition find_prev_a (a : N) (st : owners_ll) : N := todo.
-        Definition find_next_a (a : N) (st : owners_ll) : N := todo.
-    End Aux.
-
+    
     Definition result_ll := result (owners_ll * list ActionBody) error.
 
+    Section Aux.
+        Definition find_next_a (a : N) (st : owners_ll) : result N error := todo.
+        Definition find_prev_a (a : N) (st : owners_ll) : result N error := todo.
+
+        (* invariant on C_ll *)
+        Lemma find_prev_invar : forall a a_next st, 
+            find_next_a a st = Ok a_next -> 
+            exists a_prev,
+                find_prev_a a st = Ok a_prev /\
+                find_next_a a_prev st = Ok a.
+        Admitted.
+        
+        Lemma find_next_invar : forall st,
+            exists a, find_next_a SENTINEL_OWNERS st = Ok a.
+        Admitted.
+
+        Definition find_next_sentinel (st : owners_ll) : N := todo.
+
+        Lemma find_next_prev : forall a a_next st,
+            find_next_a a st = Ok a_next ->
+            Ok a = find_prev_a a_next st.
+        Admitted.
+
+        Lemma find_prev_next : forall a a_prev st,
+            find_prev_a a st = Ok a_prev ->
+            Ok a = find_next_a a_prev st.
+        Admitted.
+
+        Lemma find_prev_next' : forall a a_next st,
+            find_next_a a st = Ok a_next -> 
+            exists a_prev, find_prev_a a st = Ok a_prev.
+        Admitted.
+
+        Definition ll_insert (a : N) (st : owners_ll) : owners_ll :=
+            let a' := find_next_sentinel st in 
+            FMap.add SENTINEL_OWNERS a (FMap.add a a' st).
+        
+        Definition ll_remove (a : N) (st : owners_ll) : result owners_ll error :=
+            match FMap.find a st with
+            | None => Ok st (* returns st if a not in *)
+            | Some a_next => (* otherwise, it finds the prev owner and updates *)
+                do a_prev <- find_prev_a a st;
+                Ok (FMap.add a_prev a_next (FMap.remove a st))
+            end.
+
+        Definition ll_is_in (a : N) (st : owners_ll) : bool := 
+            match FMap.find a st with | None => false | Some _ => true end.
+        
+        
+
+        (* takes a linked list and removes the first element, if there is one *)
+        Definition ll_decrement (st : owners_ll) : owners_ll := todo.
+
+    End Aux.
+
     Definition add_owner_ll (a : N) (st : owners_ll) : result_ll :=
-        Ok (FMap.add SENTINEL_OWNERS a (FMap.add a (find_next_a a st) st), []).
-        (* match FMap.find SENTINEL_OWNERS st with
-        | None => Err error_LINK_NOT_FOUND
-        | Some a' => Ok (FMap.add SENTINEL_OWNERS a (FMap.add a a' st), [])
-        end. *)
+        if ll_is_in a st then Err error_LINK_NOT_FOUND (* no duplicates *)
+        else Ok (ll_insert a st, []). (* always succeeds *)
 
     Definition remove_owner_ll (a : N) (st : owners_ll) : result_ll :=
-        match FMap.find a st with
-        | None => Ok (st, []) (* returns st if a not in *)
-        | Some a_next => (* otherwise, it finds the prev owner and updates *)
-            let a_prev := find_prev_a a st in
-            Ok (FMap.add a_prev a_next (FMap.remove a st), [])
-        end.
+        do st' <- ll_remove a st;
+        Ok (st', []).
 
     Definition swap_owners_ll (a_fst a_snd : N) (st : owners_ll) : result_ll :=
         match FMap.find a_fst st with 
         | None => Ok (st, [])  (* returns st if a_fst not in *)
         | Some a_next =>
-            let a_prev := find_prev_a a_fst st in
+            do a_prev <- find_prev_a a_fst st;
             Ok (FMap.add a_prev a_snd (FMap.add a_snd a_next (FMap.remove a_fst st)), [])
         end.
 
@@ -161,20 +234,126 @@ Section Isomorphism.
             | [] => acc
             | a :: st' =>
                 let a' := find_next_a SENTINEL_OWNERS acc in 
-                arr_to_ll_rec st' (FMap.add SENTINEL_OWNERS a (FMap.add a a' acc))
-                (* match FMap.find SENTINEL_OWNERS acc with 
+                (* arr_to_ll_rec st' (FMap.add SENTINEL_OWNERS a (FMap.add a a' acc)) *)
+                match FMap.find SENTINEL_OWNERS acc with 
                 | Some a' => arr_to_ll_rec st' (FMap.add a a' acc)
                 | None => acc (* unreachable state TODO *)
-                end *)
+                end
             end.
 
-        Definition arr_to_ll (st : owners_arr) : owners_ll := arr_to_ll_rec st empty_linked_list.
-            
+        Definition arr_to_ll (st : owners_arr) : owners_ll :=
+            arr_to_ll_rec (List.rev st) empty_linked_list.
 
-        Definition ll_to_arr (st : owners_ll) : owners_arr := todo.
+
+        Definition ll_to_arr_rec (st : owners_ll) (acc : owners_arr) : owners_arr :=
+            match FMap.find SENTINEL_OWNERS st with
+            | None => acc
+            | Some a => 
+                match a with 
+                | 0 => acc 
+                | x => todo (* ll_to_arr_rec (ll_decrement st) (a :: acc) *)
+                end
+            end.
+        
+        Definition ll_to_arr (st : owners_ll) : owners_arr :=
+            ll_to_arr_rec st empty_array.
+
 
         (* some coherence lemmas *)
+        Lemma arr_to_ll_rev : forall st, ll_to_arr (arr_to_ll st) = st.
+        Admitted.
 
+        Lemma ll_to_arr_rev : forall st,
+            cstate_reachable C_ll st ->
+            arr_to_ll (ll_to_arr st) = st.
+        Admitted.
+
+        Lemma arr_to_ll_insert : forall a st,
+            ll_insert a (arr_to_ll st) = arr_to_ll (a :: st).
+        Admitted.
+
+        Lemma arr_to_ll_insert_inv : forall a st,
+            a :: ll_to_arr st = ll_to_arr (ll_insert a st).
+        Admitted.
+
+        Lemma arr_to_ll_remove : forall a st,
+            ll_remove a (arr_to_ll st) = 
+            Ok (arr_to_ll (List.remove N.eq_dec a st)).
+        Admitted.
+
+        Lemma ll_remove_lem : forall a st, 
+            exists x, ll_remove a st = Ok x.
+        Proof.
+            intros.
+            destruct (ll_remove a st) eqn:H_remove.
+            -   unfold ll_remove in H_remove.
+                destruct (FMap.find a st) eqn:H_found; simpl in *.
+                +   destruct (find_prev_a a st).
+                    *   now exists (FMap.add t0 n (FMap.remove a st)).
+                    *   inversion H_remove.
+                +   now exists st.
+            -   unfold ll_remove in H_remove.
+                destruct (FMap.find a st) eqn:H_found; simpl in *.
+                +   destruct (find_prev_a a st).
+                    *   inversion H_remove.
+                    *   admit.
+                +   inversion H_remove.
+        Admitted.
+
+        Lemma arr_to_ll_swap : forall a_prev a_snd a_fst n st,
+            FMap.add a_prev a_snd (FMap.add a_snd n (FMap.remove a_fst (arr_to_ll st))) =
+            arr_to_ll (map (fun o : N => if (o =? a_fst)%N then a_snd else o) st).
+        Admitted.
+
+        Lemma ll_fst_found_snd_found : forall a_fst st n,
+            FMap.find a_fst (arr_to_ll st) = Some n -> 
+            exists t, find_prev_a a_fst (arr_to_ll st) = Ok t.
+        Admitted.
+
+        (* TODO split into an invariant *)
+        Theorem arr_to_ll_no_duplicates : forall a st st' acts,
+            add_owner_arr a st = Ok (st', acts) -> 
+            (ll_is_in a (arr_to_ll st) = false).
+        Admitted.
+
+        Lemma ll_to_arr_found : forall a st,
+            ll_is_in a st = true -> 
+            exists i, in_dec N.eq_dec a (ll_to_arr st) = left i.
+        Admitted.
+
+        Lemma is_in_find_dec : forall a st i,
+            (in_dec N.eq_dec a st = left i) <->
+            (FMap.find a (arr_to_ll st) <> None).
+        Admitted.
+
+        Lemma is_in_find_dec_inv : forall a st i,
+            (in_dec N.eq_dec a (ll_to_arr st) = left i) <->
+            (FMap.find a st <> None).
+        Admitted.
+
+        Lemma swap_idempotent : forall a_fst a_snd st st' acts,
+            swap_owners_arr a_fst a_snd st = Ok (st', acts) ->
+            FMap.find a_fst (arr_to_ll st) = None ->
+            st = st'.
+        Admitted.
+
+        Lemma add_owner_ll_no_acts : forall a st st' acts,
+            add_owner_ll a st = Ok (st', acts) -> acts = [].
+        Proof.
+            intros * H_add.
+            unfold add_owner_ll in H_add.
+            destruct (ll_is_in a st) in H_add; try inversion H_add.
+            now inversion H_add.
+        Qed.
+
+        Lemma swap_owner_ll_no_acts : forall a_fst a_snd st st' acts,
+            swap_owners_ll a_fst a_snd st = Ok (st', acts) -> acts = [].
+        Proof.
+            intros * H_swap.
+            unfold swap_owners_ll in H_swap.
+            destruct (FMap.find a_fst st) in H_swap; try inversion H_swap; auto.
+            destruct (find_prev_a a_fst st) in H0; now try inversion H0.
+        Qed.
 
     End Aux.
 
@@ -188,53 +367,173 @@ Section Isomorphism.
     Definition state_morph_inv : owners_ll -> owners_arr := ll_to_arr.
 
     Section Lemmata.
+        Section Aux.
+            Lemma pair_lem { A B : Type } : forall (a a' : A) (b b' : B),
+                a = a' /\ b = b' -> (a, b) = (a', b').
+            Proof. intros. destruct H. now subst. Qed.
+        End Aux.
+
         (* some coherence lemmas for init *)
         Lemma empty_coh : state_morph empty_array = empty_linked_list.
-        Admitted.
+        Proof.
+            unfold state_morph, empty_array, empty_linked_list.
+            unfold arr_to_ll.
+            simpl.
+            now unfold empty_linked_list.
+        Qed.
         
         Lemma empty_coh_rev : state_morph_inv empty_linked_list = empty_array.
-        Admitted.
+        Proof.
+            unfold state_morph_inv, empty_array, empty_linked_list.
+            unfold ll_to_arr, ll_to_arr_rec, SENTINEL_OWNERS.
+            replace (FMap.find 0 (FMap.add 0 0 FMap.empty))
+            with (Some 0) by auto.
+            now unfold empty_array.
+        Qed.
 
         (* some coherence lemmas for recv *)
         Lemma add_owner_coh : forall a st st' acts,
             add_owner_arr a st = Ok (st', acts) ->
             add_owner_ll a (state_morph st) = Ok (state_morph st', acts).
-        Admitted.
+        Proof.
+            intros * H_in.
+            unfold add_owner_arr, add_owner_ll, state_morph in *.
+            replace (ll_is_in a (arr_to_ll st)) with false
+            by (apply arr_to_ll_no_duplicates in H_in; now symmetry).
+            apply f_equal.
+            apply pair_lem.
+            split.
+            -   destruct (in_dec N.eq_dec a st) in H_in; try inversion H_in.
+                unfold ll_insert.
+                apply arr_to_ll_insert.
+            -   symmetry.
+                now apply (add_owner_arr_no_acts a st st' acts).
+        Qed.
 
         Lemma add_owner_coh' : forall a st e,
             add_owner_arr a st = Err e ->
             add_owner_ll a (state_morph st) = Err e.
-        Admitted.
+        Proof.
+            intros * H_in.
+            unfold add_owner_arr, add_owner_ll, state_morph in *.
+            replace (ll_is_in a (arr_to_ll st)) with true.
+            -   destruct (in_dec N.eq_dec a st) in H_in; now try inversion H_in.
+            -   unfold ll_is_in.
+                destruct (FMap.find a (arr_to_ll st)) eqn:H_found; auto.
+                pose proof is_in_find_dec as H_is_in.
+                destruct (in_dec N.eq_dec a st) eqn:H_found'; try inversion H_in.
+                apply H_is_in in H_found'.
+                rewrite H_found in H_found'.
+                contradiction.
+        Qed.
 
         Lemma remove_owner_coh : forall a st st' acts,
             remove_owner_arr a st = Ok (st', acts) ->
             remove_owner_ll a (state_morph st) = Ok (state_morph st', acts).
-        Admitted.
+        Proof.
+            intros * H_remove.
+            unfold remove_owner_arr, remove_owner_ll, state_morph in *.
+            simpl.
+            inversion H_remove as [[H_r0 H_r1]].
+            destruct (ll_remove a (arr_to_ll st)) eqn:H_remove'.
+            -   f_equal.
+                apply pair_lem.
+                split; auto.
+                now rewrite arr_to_ll_remove in H_remove'.
+            -   pose proof (ll_remove_lem a (arr_to_ll st)).
+                destruct H as [x H].
+                rewrite H in H_remove'.
+                now inversion H_remove'.
+        Qed.
 
         Lemma remove_owner_coh' : forall a st e,
             remove_owner_arr a st = Err e ->
             remove_owner_ll a (state_morph st) = Err e.
-        Admitted.
+        Proof.
+            intros * H_remove.
+            unfold remove_owner_arr, remove_owner_ll, state_morph in *.
+            simpl.
+            destruct (ll_remove a (arr_to_ll st)) eqn:H_remove'.
+            -   destruct (FMap.find a (arr_to_ll st)) eqn:H_find.
+                +   now inversion H_remove.
+                +   now inversion H_remove.
+            -   now inversion H_remove.
+        Qed.
 
         Lemma swap_owners_coh : forall a_fst a_snd st st' acts,
             swap_owners_arr a_fst a_snd st = Ok (st', acts) ->
             swap_owners_ll a_fst a_snd (state_morph st) = Ok (state_morph st', acts).
-        Admitted.
+        Proof.
+            intros * H_swap.
+            apply swap_owner_arr_no_acts in H_swap as H_acts.
+            rewrite H_acts in *.
+            unfold swap_owners_ll.
+            destruct (FMap.find a_fst (state_morph st)) eqn:H_fst_found.
+            (* case where a_fst is there *)
+            -   simpl.
+                unfold state_morph in *.
+                apply ll_fst_found_snd_found in H_fst_found as H_prev_found.
+                destruct H_prev_found as [a_prev H_prev_found].
+                rewrite H_prev_found.
+                f_equal.
+                apply pair_lem.
+                split.
+                2:{ pose proof (add_owner_arr_no_acts).
+                    now apply swap_owner_arr_no_acts in H_swap. }
+                unfold swap_owners_arr in H_swap.
+                inversion H_swap as [H_res].
+                now apply arr_to_ll_swap.
+            (* case where a_fst is not there *)
+            -   unfold state_morph in *.
+                apply swap_idempotent in H_swap; auto.
+                now rewrite H_swap.
+        Qed.
 
         Lemma swap_owners_coh' : forall a_fst a_snd st e,
             swap_owners_arr a_fst a_snd st = Err e ->
             swap_owners_ll a_fst a_snd (state_morph st) = Err e.
-        Admitted.
+        Proof.
+            intros * H_swap.
+            pose proof (swap_always_succeeds a_fst a_snd st) as H_success.
+            destruct H_success as [st' H_success].
+            rewrite H_success in H_swap.
+            inversion H_swap.
+        Qed.
 
         Lemma add_owner_coh_inv : forall a st st' acts,
             add_owner_ll a st = Ok (st', acts) ->
             add_owner_arr a (state_morph_inv st) = Ok (state_morph_inv st', acts).
-        Admitted.
+        Proof.
+            intros * H_in.
+            apply add_owner_ll_no_acts in H_in as H_acts.
+            rewrite H_acts in *. clear H_acts.
+            unfold add_owner_arr, add_owner_ll, state_morph_inv in *.
+            destruct (ll_is_in a st) eqn:H_found.
+            inversion H_in.
+            unfold ll_is_in in H_found.
+            destruct (FMap.find a st) eqn:H_found'; try inversion H_found.
+            destruct (in_dec N.eq_dec a (ll_to_arr st)) eqn:H_in'.
+            {   apply is_in_find_dec_inv in H_in'.
+                now rewrite H_found' in H_in'. }
+            f_equal.
+            apply pair_lem.
+            split; auto.
+            inversion H_in as [H_insert_st].
+            now apply arr_to_ll_insert_inv.
+        Qed.
 
         Lemma add_owner_coh'_inv : forall a st e,
             add_owner_ll a st = Err e ->
             add_owner_arr a (state_morph_inv st) = Err e.
-        Admitted.
+        Proof.
+            intros * H_in.
+            unfold add_owner_arr, add_owner_ll, state_morph_inv in *.
+            destruct (ll_is_in a st) eqn:H_found; try inversion H_in.
+            rewrite H0. clear H0.
+            apply ll_to_arr_found in H_found.
+            destruct H_found as [i H_found].
+            now rewrite H_found.
+        Qed.
 
         Lemma remove_owner_coh_inv : forall a st st' acts,
             remove_owner_ll a st = Ok (st', acts) ->
@@ -260,6 +559,7 @@ Section Isomorphism.
         Lemma state_morph_iso : forall st, state_morph (state_morph_inv st) = st.
         Admitted.
 
+        (* this is true under invariants *)
         Lemma state_morph_iso_inv : forall st, state_morph_inv (state_morph st) = st.
         Admitted.
 
@@ -355,9 +655,29 @@ Section Isomorphism.
     Theorem iso_arr_all : is_iso_cm f_inv f.
     Proof. apply iso_cm_symmetric. apply iso_ll_arr. Qed.
 
-    Theorem contracts_isomorphic : contracts_isomorphic C_arr C_ll.
+    Theorem bisim_arr_ll : contracts_isomorphic C_arr C_ll.
     Proof. exists f, f_inv. apply iso_ll_arr. Qed.
 
 End Isomorphism.
+
+
+Section Specification.
+
+    Definition no_duplciates_arr (st : owners_arr) : Prop := NoDup st.
+
+    Definition no_duplciates_ll (st : owners_ll) : Prop :=
+        todo. (* you can cycle through the list and return to SENTINEL *)
+
+    (* proved by contract induction *)
+    Theorem no_duplciates (cstate : owners_arr) :
+        cstate_reachable C_arr cstate -> no_duplciates_arr cstate.
+    Admitted.
+
+    (* proved by morphism induction *)
+    Theorem no_duplciates' (cstate : owners_ll) : 
+        cstate_reachable C_ll cstate -> no_duplciates_ll cstate.
+    Admitted.
+
+End Specification.
 
 End ContractOptimization.
